\subsection*{Exercise 02 (Gapry)}

\begin{flushleft}
Define a function $f(n) = \sqrt{n^2 + n} - n$, 
$\lim\limits_{n \to \infty}\sqrt{n^2 + n} - n = \lim\limits_{n \to \infty}f(n)$

Let's rationalize the function $f(n)$
\begin{flalign*}
f(n) &= \sqrt{n^2 + n} - n                                                  &\\
     &= \frac{(\sqrt{n^2 + n} - n)(\sqrt{n^2 + n} + n)}{\sqrt{n^2 + n} + n} &\\
     &= \frac{(\sqrt{n^2 + n})^2 - n^2}{\sqrt{n^2 + n} + n}                 &\\
     &= \frac{n^2 + n - n^2}{\sqrt{n^2 + n} + n}                            &\\
     &= \frac{n}{\sqrt{n^2 + n} + n}                                        &\\
     &= \frac{\frac{n}{n}}{\frac{\sqrt{n^2 + n} + n}{n}}                    &\\
     &= \frac{1}{\frac{\sqrt{n^2 + n}}{n} + \frac{n}{n}}                    &\\
     &= \frac{1}{\sqrt{\frac{n^2 + n}{n^2}} + 1}                            &\\
     &= \frac{1}{\sqrt{\frac{n^2}{n^2} + \frac{n}{n^2}} + 1}                &\\
     &= \frac{1}{\sqrt{1 + \frac{1}{n}} + 1}                                &\\
\end{flalign*}

We find that $\sqrt{n^2 + n} - n = f(n) = \frac{1}{\sqrt{1 + \frac{1}{n}} + 1}$.

Therefore, we can conclude that
$\lim\limits_{n \to \infty} \sqrt{n^2 + n} - n = 
 \lim\limits_{n \to \infty} f(n)               =
 \lim\limits_{n \to \infty} \frac{1}{\sqrt{1 + \frac{1}{n}} + 1}
$. 

According to the definition 3.1 (a), 
we know that $\lim\limits_{n \to \infty} \frac{1}{n} = 0$, 
hence $\lim\limits_{n \to \infty} \frac{1}{\sqrt{1 + \frac{1}{n}} + 1} = 
\frac{1}{\sqrt{1 + 0} + 1} = \frac{1}{2}$
\end{flushleft}
