\subsection*{Exercise 11 (Gapry)}
If the distance function can construct a metric space, it will satisfy the following condition: For any \(x,\ y,\ z\) in set \(X\):
\begin{enumerate}
\item \(d(x,\ x) = 0\)
\item \(d(x,\ y) > 0\) if \(x \neq y\)
\item \(d(x,\ y) = d(y,\ x)\)
\item \(d(x,\ y) \leq d(x,\ z) + d(z,\ y)\)
\end{enumerate}

\subsubsection*{Part 01: Analyze $d_1(x,\ y) = (x - y)^2$}
\begin{flalign*}
d_1(x,\ y) &= (x - y)^2                               &\\
           &= (x - z + z - y)^2                       &\\
           &= ((x - z) + (z - y))^2                   &\\
           &= (x - z)^2 + 2(x - z)(z - y) + (z - y)^2 &\\ 
           &= (x - z)^2 + (z - y)^2 + 2(x - z)(z - y) &\\ 
           &= d_1(x,\ z) + d_1(z,\ y) + 2(x - z)(z - y)
\end{flalign*}

\begin{flushleft}
If $x > z$ and $z > y$, $d_1(x,\ y)$ can't satisfy the 4th condition.
\end{flushleft}

\subsubsection*{Part 02: Analyze $d_2(x,\ y) = \sqrt{|x - y|}$}

\begin{enumerate}
\item \(d_2(x,\ x) = \sqrt{|x - x|} = 0\)
\item \(d_2(x,\ y) = \sqrt{|x - y|} > 0\) if \(x \neq y\)
\item \(d_2(x,\ y) = \sqrt{|x - y|} = \sqrt{|y - x|} = d_2(y,\ x)\)
\end{enumerate}

\begin{flushleft}
According Theorem 1.37(f), we know $|x - y| \le |x - z| + |z - y|$ is true. Hence, we have the following inference:
\begin{flalign*}
                |x - y| &\le |x - z| + |z - y|               &\\
\implies \sqrt{|x - y|} &\le \sqrt{|x - z|} + \sqrt{|z - y|} &\\
\implies     d_2(x,\ y) &\le d_2(x,\ z) + d_2(z,\ y)
\end{flalign*}

Since $d_2(x,\ y)$ can satisfy the all conditions, it is a metric space.
\end{flushleft}

\subsubsection*{Part 03: Analyze $d_3(x,\ y) = |x^2 - y^2|$}
\begin{flushleft}
Let's claim $y = -x$, $|x^2 - y^2| = |x^2 - (-x)^2| = 0$ \\
$d_3(x,\ y)$ can't satisfy the 2nd condition.
\end{flushleft}

\subsubsection*{Part 04: Analyze $d_4(x,\ y) = |x - 2y|$}
\begin{flushleft}
$d_4(x,\ y) = |x - 2y|$, $d_4(y,\ x) = |y - 2x|$
Since $d_4(x,\ y) \neq d_4(y,\ x)$, $d_4(x,\ y)$ can't satisfy the 3rd condition.
\end{flushleft}

\subsubsection*{Part 05: Analyze $d_5(x,\ y) = \frac{|x - y|}{1 + |x - y|}$}

\begin{enumerate}
\item \(d_5(x,\ x) = \frac{|x - x|}{1 + |x - x|} = 0\)
\item \(d_5(x,\ y) = \frac{|x - y|}{1 + |x - y|} > 0\) if \(x \neq y\)
\item \(d_5(x,\ y) = \frac{|x - y|}{1 + |x - y|} = \frac{|y - x|}{1 + |y - x|} = d_5(y,\ x)\)
\end{enumerate}

We do the following inference:
\begin{flalign*}
                                       d_5(x,\ y) &= \frac{|x - y|}{1 + |x - y|}         &\\
d_5(x,\ y)(1 + |x - y|)(1 + |x - z|)(1 + |z - y|) &= |x - y|(1 + |x - z|)(1 + |z - y|)   &\\
                                       d_5(x,\ z) &= \frac{|x - z|}{1 + |x - z|}         &\\
d_5(x,\ z)(1 + |x - y|)(1 + |x - z|)(1 + |z - y|) &= |x - z|(1 + |x - y|)(1 + |z - y|)   &\\
                                       d_5(z,\ y) &= \frac{|z - y|}{1 + |z - y|}         &\\
d_5(z,\ y)(1 + |x - y|)(1 + |x - z|)(1 + |z - y|) &= |z - y|(1 + |x - y|)(1 + |x - z|)   &\\
                          d_5(x,\ z) + d_5(z,\ y) &= (1 + |x - y|)(|x - z|(1 + |z - y|) 
                                                                 + |z - y|(1 + |x - z|)) &\\
                                                  &= (1 + |x - y|)(|z - y|(1 + |x - z|) 
                                                                 + |x - z|(1 + |z - y|)) &\\
                                          |x - y| &\le 1 + |x - y|                       &\\
                                      1 + |x - z| &\le |z - y|(1 + |x - z|)              &\\
                                      1 + |z - y| &\le |x - z|(1 + |z - y|)              &\\
                                       d_5(x,\ y) &\le d_5(x,\ z) + d_5(z,\ y)
\end{flalign*}
\begin{flushleft}
Since $d_5(x,\ y)$ can satisfy the all conditions, it is a metric space.
\end{flushleft}